Fixed the highest var comp proof. Disastrous. Also fixed some mistakes in the comp_program (which were preventing the previous theorem from being proven.) Three execution from states remain, plus the execution from state for the entire program. Once that is completed, the first part of the big proof should be immediate.

Loop/Basic.lean
@@ -976,25 +976,36 @@ def comp_program (g : Fin n → VectNat m → Nat) (_ : cleanly_computes p_f f) 
       ++ clear_X_j_to_X_n_plus_j 1 m
       ++ p_f
       ++ setup_X_j_to_X_n_plus_j (offset_comp (m + 1) p_g p_f) 1 m
-      ++ clear_Z_0_to_Z_n (offset_comp m p_g p_f + 1) m
+      ++ clear_Z_0_to_Z_n (offset_comp (m + 1) p_g p_f + 1) m
   | n + 1 => match m with
     | 0 =>
-         compute_store_all_succ_n_g n m p_g p_f (offset_comp m p_g p_f + m)
-      ++ setup_X_j_to_X_n_plus_j (offset_comp m p_g p_f + m) 1 n
-      ++ clear_Z_0_to_Z_n (offset_comp m p_g p_f + m + 1) n
+         compute_store_all_succ_n_g n 0 p_g p_f (offset_comp 0 p_g p_f)
+      ++ setup_X_j_to_X_n_plus_j (offset_comp 0 p_g p_f) 1 n
+      ++ clear_Z_0_to_Z_n (offset_comp 0 p_g p_f + 1) n
       ++ p_f
       ++ clear_X_j_to_X_n_plus_j 1 n
     | m + 1 =>
          store_X_1_to_X_succ_n (offset_comp (m + 1) p_g p_f + 1) m
-      ++ compute_store_all_succ_n_g n m p_g p_f (offset_comp m p_g p_f + m)
+      ++ compute_store_all_succ_n_g n (m + 1) p_g p_f (offset_comp (m + 1) p_g p_f + (m + 1))
       ++ clear_X_j_to_X_n_plus_j 1 m
-      ++ setup_X_j_to_X_n_plus_j (offset_comp m p_g p_f + m) 1 n
-      ++ clear_Z_0_to_Z_n (offset_comp m p_g p_f + m + 1) n
+      ++ setup_X_j_to_X_n_plus_j (offset_comp (m + 1) p_g p_f + (m + 1)) 1 n
+      ++ clear_Z_0_to_Z_n (offset_comp (m + 1) p_g p_f + (m + 1) + 1) n
       ++ p_f
       ++ clear_X_j_to_X_n_plus_j 1 n
       ++ setup_X_j_to_X_n_plus_j (offset_comp (m + 1) p_g p_f) 1 m
-      ++ clear_Z_0_to_Z_n (offset_comp m p_g p_f + 1) m
+      ++ clear_Z_0_to_Z_n (offset_comp (m + 1) p_g p_f + 1) m
 
+def offset_comp_lemma (m : Nat) (p_g : Fin (n + 1) → Program) (p_f : Program) :
+    offset_comp m p_g p_f ≥ offset_comp m (fun i => p_g i.succ) p_f := by
+  dsimp [offset_comp]
+  have h_1 := max_le_lemma n m (n + 1) m (Nat.le_succ n) (Nat.le_refl m)
+  have h_2 : highest_var_p_g p_g ≥ highest_var_p_g fun i => p_g i.succ := by
+    have : highest_var_p_g p_g = max (highest_var (p_g 0)) (highest_var_p_g (fun i => p_g i.succ)) := rfl
+    rewrite [this]
+    simp
+  have h_3 := max_le_lemma (highest_var p_f) (highest_var_p_g fun i => p_g i.succ)
+      (highest_var p_f) (highest_var_p_g p_g) (Nat.le_refl _) h_2
+  exact max_le_lemma _ _ _ _ h_1 h_3
 
 def highest_var_compute_store_all_succ_n_g_lemma (n m k : Nat) (p_g : Fin (n + 1) → Program) (p_f : Program)
     : ∀ x : Nat, x ≥ offset_comp m p_g p_f →
@@ -1036,19 +1047,7 @@ def highest_var_compute_store_all_succ_n_g_lemma (n m k : Nat) (p_g : Fin (n + 1
       generalize highest_var (compute_store_all_succ_n_g n m (fun i ↦ p_g i.succ) p_f (x + 1)) = t
       apply Nat.add_max_add_right
     rewrite [Nat.add_assoc]
-    have : offset_comp m p_g p_f ≥ offset_comp m (fun i => p_g i.succ) p_f := by
-      dsimp [offset_comp]
-      have h_1 : max (n + 1 + 1) m ≥ max (n + 1) m :=
-        max_le_lemma (n + 1) m (n + 1 + 1) m (Nat.le_succ (n + 1)) (Nat.le_refl m)
-      have h_2 : highest_var_p_g p_g ≥ highest_var_p_g fun i ↦ p_g i.succ := by
-        have : highest_var_p_g p_g = max (highest_var (p_g 0)) (highest_var_p_g (fun i => p_g i.succ)) := rfl
-        rewrite [this]
-        simp
-      have h_3 : max (highest_var p_f) (highest_var_p_g p_g)
-          ≥ max (highest_var p_f) (highest_var_p_g fun i ↦ p_g i.succ) :=
-         max_le_lemma (highest_var p_f) (highest_var_p_g fun i ↦ p_g i.succ)
-          (highest_var p_f) (highest_var_p_g p_g) (Nat.le_refl _) h_2
-      exact max_le_lemma _ _ _ _ h_1 h_3
+    have : offset_comp m p_g p_f ≥ offset_comp m (fun i => p_g i.succ) p_f := offset_comp_lemma _ _ _
     have h'' := Nat.le_trans this x_h
     rewrite [n_ih (1 + k) (fun i => p_g i.succ) x h'']
     rewrite [←Nat.add_assoc]
@@ -1085,7 +1084,7 @@ def highest_var_compute_store_all_succ_n_g (n m : Nat) (p_g : Fin (n + 1) → Pr
     have := Nat.le_trans (@highest_var_p_g_ge_highest_var_p_g_i _ p_g 0) this
     have := @Nat.le_add_right_of_le _ _ 1 this
     rewrite [Nat.max_eq_right this]
-    have : offset_comp m (fun i ↦ p_g i.succ) p_f ≤ x  := by sorry
+    have : offset_comp m (fun i => p_g i.succ) p_f ≤ x :=  Nat.le_trans (offset_comp_lemma m p_g p_f) x_h
     have := n_ih (fun i => p_g i.succ) (x + 1) (Nat.le_trans this (Nat.le_succ x))
     rewrite [this]
     simp_arith
@@ -1129,39 +1128,58 @@ def highest_var_comp_program (g : Fin n → VectNat m → Nat) (f_h : cleanly_co
         exact Nat.max_eq_left this
 
       rewrite [this]
-      rewrite [Nat.max_self]
-      have : max (offset_comp (m + 1) p_g p_f + 1 + m) (offset_comp m p_g p_f + 1 + m)
-          = offset_comp (m + 1) p_g p_f + 1 + m := by
-        suffices h : offset_comp (m + 1) p_g p_f ≥ offset_comp m p_g p_f from by
-          have := Nat.add_le_add_right h (1 + m)
-          rewrite [←Nat.add_assoc, ←Nat.add_assoc] at this
-          exact Nat.max_eq_left this
-        dsimp [offset_comp]
-        rewrite [Nat.zero_max, Nat.zero_max]
-        generalize max (highest_var p_f) (highest_var_p_g p_g) = x
-        simp
-        cases (Nat.decLe m x )
-        case isFalse h =>
-          apply Or.intro_left
-          have := Nat.gt_of_not_le h
-          have : x + 1 ≤ m := this
-          have := @Nat.le_add_right_of_le _ _ 2 this
-          exact Nat.le_of_succ_le_succ this
-        case isTrue h =>
-          apply Or.intro_right
-          assumption
-
-      rewrite [this]
-      rw [Nat.add_comm m, Nat.add_assoc]
+      rw [Nat.max_self, Nat.max_self, Nat.add_comm m 1, ←Nat.add_assoc]
   case succ n =>
     cases m
     case zero =>
       dsimp [comp_program, highest_var]
       rewrite [highest_var_setup, highest_var_clear, highest_var_clear_Z]
-
-      sorry
+      have := Nat.add_zero (offset_comp 0 p_g p_f)
+      rewrite [this.symm]
+      rewrite [highest_var_compute_store_all_succ_n_g]
+      rewrite [this]
+      have h : max (n + 1) (offset_comp 0 p_g p_f + n + 1) = offset_comp 0 p_g p_f + n + 1 := by simp_arith
+      rewrite [h]
+      rewrite [←Nat.add_assoc, Nat.max_self]
+      have : offset_comp 0 p_g p_f + n + 1 = offset_comp 0 p_g p_f + 1 + n:= by simp_arith
+      rewrite [this, Nat.max_self, this.symm]
+      have : max (offset_comp 0 p_g p_f + n + 1) (highest_var p_f) = offset_comp 0 p_g p_f + n + 1 := by
+        have : highest_var p_f ≤ offset_comp 0 p_g p_f := by simp_arith [offset_comp]
+        have := @Nat.le_add_right_of_le _  _ (n + 1) this
+        rewrite [←Nat.add_assoc] at this
+        rw [Nat.max_eq_left this]
+      rw [this, Nat.max_comm, h]
     case succ m =>
-      sorry
+      dsimp [comp_program, highest_var]
+      rewrite [highest_var_compute_store_all_succ_n_g]
+      repeat rewrite [highest_var_store]
+      repeat rewrite [highest_var_clear]
+      repeat rewrite [highest_var_clear_Z]
+      repeat rewrite [highest_var_setup]
+      rewrite [Nat.add_assoc, Nat.add_comm 1 m]
+      rewrite [Nat.add_assoc _ n 1]
+      rewrite [Nat.add_assoc _ m 1]
+      have l : ∀ a b : Nat, max a (b + a) = b + a := by simp_arith
+      have l' : ∀ a b : Nat, max a (a + b) = a + b := by simp_arith
+      rewrite [l, l, l']
+      rewrite [Nat.max_comm _ (m + 1)]
+      rewrite [Nat.add_assoc _ (m + 1), Nat.add_comm (m + 1), ←Nat.add_assoc _ _ (m + 1)]
+      rewrite [l, Nat.max_self]
+      rewrite [Nat.add_assoc _ 1 n, Nat.add_comm 1 n, Nat.add_assoc _ _ (n + 1),
+        Nat.add_comm (m + 1) (n + 1), ←Nat.add_assoc _ (n + 1)]
+      rewrite [Nat.max_self]
+      have : max (offset_comp (m + 1) p_g p_f + (n + 1) + (m + 1)) (highest_var p_f)
+          = offset_comp (m + 1) p_g p_f + (n + 1) + (m + 1) := by
+        have : highest_var p_f ≤ offset_comp (m + 1) p_g p_f := by simp [offset_comp]
+        have h := @Nat.le_add_right_of_le _ _ ((n + 1) + (m + 1)) this
+        have : n + 1 + (m + 1) = (n + 1) + (m + 1) := by simp_arith
+        rewrite [this, ←Nat.add_assoc] at h
+        exact Nat.max_eq_left h
+      rewrite [this, Nat.max_comm _ (n + 1)]
+      rewrite [Nat.add_assoc _ (n + 1), Nat.add_comm (n + 1) _, ←Nat.add_assoc _ _ (n + 1)]
+      rewrite [l]
+      rewrite [Nat.max_comm (offset_comp (m + 1) p_g p_f + (m + 1) + (n + 1))]
+      rw [l', Nat.max_comm, l']
 
 -- 1. def execution_from_state_comp_store_succ_m_inputs
 -- 2. def execution_from_state_comp_compute_store_succ_n_g
@@ -1173,14 +1191,30 @@ def highest_var_comp_program (g : Fin n → VectNat m → Nat) (f_h : cleanly_co
 -- 8. def execution_from_state_comp_setup_succ_m_inputs
 -- def execution_from_state_comp_clear_succ_m_z
 
--- theorem comp_is_loop_computable_cleanly (g : Fin n → VectNat m → Nat) :
---       loop_computable_cleanly f
---     → (∀ i, loop_computable_cleanly (g i))
---     → loop_computable_cleanly fun a => f (Vector.ofFn fun i => g i a) := by
---   intro ⟨p_f, f_h⟩ g_h
---   have ⟨p_g, g_h⟩ := forall_exists_function g g_h
+theorem comp_is_loop_computable_cleanly (g : Fin n → VectNat m → Nat) :
+      loop_computable_cleanly f
+    → (∀ i, loop_computable_cleanly (g i))
+    → loop_computable_cleanly fun a => f (Vector.ofFn fun i => g i a) := by
+  intro ⟨p_f, f_h⟩ g_h
+  have ⟨p_g, g_h⟩ := forall_exists_function g g_h
+  exists comp_program g f_h p_g g_h
+  intro v
+  rewrite [highest_var_comp_program]
+  have : offset_comp m p_g p_f + m + n - m = (offset_comp m p_g p_f - m) + (m + n) := by
+    rewrite [Nat.add_assoc , Nat.add_comm m n, ←Nat.add_assoc]
+    rewrite [Nat.add_sub_cancel]
+    have : offset_comp m p_g p_f ≥ m := by simp_arith [offset_comp]
+    rewrite [Nat.add_comm n m, ←Nat.add_assoc]
+    rw [Nat.sub_add_cancel this]
+  rewrite [this]
+  simp_arith
+  rewrite [←append_zeros_addition (offset_comp m p_g p_f - m) (m + n)
+     (offset_comp m p_g p_f - m + (m + n)) rfl]
+  -- rewrite [←append_zeros_addition m n (m + n) rfl]
+  repeat rewrite [←List.append_assoc]
+  repeat rewrite [←List.cons_append]
 
---   sorry
+  sorry
 
 end comp_is_loop_computable_cleanly_proof
 
